Linglib.lean
@@ -119,6 +119,7 @@ import Linglib.Core.Data.List.Chain
 import Linglib.Core.Data.List.Destutter
 import Linglib.Core.Data.List.DropRight
 import Linglib.Core.Data.List.Factors
+import Linglib.Core.Data.List.Fold
 import Linglib.Core.Data.List.TakeDrop
 import Linglib.Core.Data.RoseTree.Basic
 import Linglib.Core.Data.RoseTree.Get
